LinearScan/ssreflect.hs
@@ -3,6 +3,7 @@ module LinearScan.Ssreflect where
 
 import qualified Prelude
 import qualified Data.IntMap
+import qualified Data.IntSet
 import qualified Data.List
 import qualified Data.Ord
 import qualified Data.Functor.Identity
